changed conservativity proof and notion of subsystem

theories/IsCanonical.v
@@ -11,112 +11,77 @@ Import ListNotations.
 (* predicado para termos canónicos *)
 
 Inductive is_canonical: term -> Prop :=
-| cVar (x: var) : is_canonical (Var x)
-| cLam (t: {bind term}) : is_canonical t -> is_canonical (Lam t)                                                      
+| cVar (x: var) :
+  is_canonical (Var x)
+
+| cLam (t: {bind term}) :
+  is_canonical t -> is_canonical (Lam t)
+
 | cVarApp (x: var) (u: term) (l: list term) :
-  is_canonical u -> is_canonical_list l -> is_canonical (mApp (Var x) u l)
+  is_canonical u -> is_canonical_list l ->
+  is_canonical (mApp (Var x) u l)
+
 | cLamApp (t: {bind term}) (u: term) (l: list term) :
-  is_canonical t -> is_canonical u -> is_canonical_list l -> is_canonical (mApp (Lam t) u l)
+  is_canonical t -> is_canonical u -> is_canonical_list l ->
+  is_canonical (mApp (Lam t) u l)
 
 with is_canonical_list: list term -> Prop :=
 | cNil : is_canonical_list []
-| cCons (u: term) (l: list term) : is_canonical u -> is_canonical_list l -> is_canonical_list (u::l).
 
-Hint Constructors is_canonical is_canonical_list : core.
+| cCons (u: term) (l: list term) :
+  is_canonical u -> is_canonical_list l ->
+  is_canonical_list (u::l).
+
+Local Hint Constructors is_canonical is_canonical_list : core.
 
 Scheme sim_is_canonical_ind := Induction for is_canonical Sort Prop
   with sim_is_canonical_list_ind := Induction for is_canonical_list Sort Prop.  
 
 Combined Scheme mut_is_canonical_ind from sim_is_canonical_ind, sim_is_canonical_list_ind.
 
+(* definition of @ operation in λm *)
+(* ------------------------------- *)
+
 Definition app (v u: term) (l: list term) : term :=
   match v with
-  | Var x => mApp v u l
-  | Lam t => mApp v u l
+  | Var x        => mApp v u l
+  | Lam t        => mApp v u l
   | mApp t u' l' => mApp t u' (l' ++ (u::l))
   end.
 
-Lemma list_append_is_closed :
-  forall l1 l2, is_canonical_list l1 -> is_canonical_list l2 -> is_canonical_list (l1++l2).
+(* lets prove that the image of h is canonical *)
+(* ------------------------------------------- *)
+
+Lemma list_append_is_canonical l1 l2:
+  is_canonical_list l1 -> is_canonical_list l2 ->
+  is_canonical_list (l1++l2).
 Proof.
-  intros l1 l2 il1 il2.
+  intros il1 il2.
   induction l1 ; simpl ; inversion il1 ; subst ; auto.
 Qed.
 
-Hint Resolve list_append_is_closed : core.
-
-Lemma app_is_closed :
-  forall t u l, is_canonical t -> is_canonical u -> is_canonical_list l ->
-           is_canonical (app t u l).
+Lemma app_is_canonical t u l :
+  is_canonical t -> is_canonical u -> is_canonical_list l ->
+  is_canonical (app t u l).
 Proof.
-  intros t u l it iu il.
-  destruct t as [x | t | v u' l'] ; asimpl ;
-    try inversion it ; subst ; auto.
+  intros it iu il.
+  destruct t as [x | t | v u' l'] ; asimpl ; auto.
+  - inversion it ; subst. auto.
+  - inversion it ; subst.
+    + constructor ; try easy.
+      * apply list_append_is_canonical ; auto.
+    + constructor ; try easy.
+      * apply list_append_is_canonical ; auto.
 Qed.
+  
+(* app does H reduction *)
+(* -------------------- *)
 
-Hint Resolve app_is_closed : core.
-          
-Instance Subst_Canonical : Subst term :=
-  (fix inst (σ: var -> term) (s: term) : term :=
-     match s with
-     | Var x => σ x
-     | Lam t => Lam (inst (up σ) t)
-     | mApp v u l => app (inst σ v) (inst σ u) (mmap (inst σ) l)
-   end).
-
-Notation "s .{ σ }" := (Subst_Canonical σ s)                              
-  (at level 2, σ at level 200, left associativity,
-    format "s .{ σ }" ) : subst_scope.
-                        
-Notation "l ..{ σ }" := (mmap (Subst_Canonical σ) l)
-  (at level 2, σ at level 200, left associativity,
-    format "l ..{ σ }" ) : subst_scope.                             
-
-Existing Instance Subst_term.
-
-Definition is_canonical_subst (σ: var -> term) :=
-  forall x, is_canonical (σ x).
-
-Hint Unfold is_canonical_subst : core.
-
-Lemma ren_is_closed :
-  (forall t, is_canonical t -> forall ξ, is_canonical t.[ren ξ])
-  /\
-  (forall l, is_canonical_list l -> forall ξ, is_canonical_list l..[ren ξ]).
+Theorem app_is_multistep_H t u l :
+  multistep_H (mApp t u l) (app t u l).
 Proof.
-  apply mut_is_canonical_ind ; intros ; asimpl ; auto.
-Qed. 
-
-Lemma up_subst_is_closed :
-  forall σ, is_canonical_subst σ -> is_canonical_subst (up σ).
-Proof.
-  intros σ H. autounfold.
-  destruct x ; asimpl ; try easy.
-  - now apply ren_is_closed.
+  destruct t ; asimpl ; try constructor.
+  - apply rt1n_trans with (mApp t1 t2 (l0 ++ u :: l)).
+    + now constructor.
+    + now constructor.
 Qed.
-
-Local Hint Resolve up_subst_is_closed : core.
-
-Theorem subst_is_closed :
-  (forall t, is_canonical t -> forall σ, is_canonical_subst σ -> is_canonical t.{σ})
-  /\
-  (forall l, is_canonical_list l -> forall σ, is_canonical_subst σ -> is_canonical_list l..{σ}).
-Proof.
-  apply mut_is_canonical_ind ; intros ; asimpl ; auto.
-Qed.
-          
-(* Redução em termos canónicos *)
-(* --------------------------- *)
-
-Inductive β1' : relation term :=
-| Can_Step_Beta1 (t: {bind term}) (u t': term):
-  t' = t.{u .: ids} ->
-  β1' (mApp (Lam t) u []) t'.
-
-Inductive β2' : relation term :=
-| Can_Step_Beta2 (t: {bind term}) (u u' t': term) (l: list term):
-  t' = app t.{u .: ids} u' l ->
-  β2' (mApp (Lam t) u (u'::l)) t'.
-
-Definition step_can := comp (union _ β1' β2').
-Definition step_can' := comp' (union _ β1' β2').
