theories/Conservativeness.v
@@ -1,56 +1,18 @@
 From Coq Require Import List.
 From Coq Require Import Relations.Relation_Definitions.
 From Coq Require Import Relations.Relation_Operators.
+Require Import MyRelations.
 
 Require Import Autosubst.Autosubst.
-Require Import LambdaM Canonical IsCanonical CanonicalIsomorphism.
+Require Import LambdaM Canonical.
+Require Import IsCanonical CanonicalIsomorphism.
 
 Import ListNotations.
 
-Proposition multistep_trans (A: Type) (R: relation A):
-  forall x y z, clos_refl_trans_1n _ R x y -> clos_refl_trans_1n _ R y z ->
-           clos_refl_trans_1n _ R x z.
-Proof.                                                  
-  intros.
-  induction H ; try easy.
-  - apply rt1n_trans with y ; try easy.
-    + now apply IHclos_refl_trans_1n. 
-Qed.
-
-Lemma mApp_multistep_to_app :
-  forall t u l, LambdaM.multistep (mApp t u l) (app t u l).
-Proof.
-  destruct t ; intros ; asimpl ; try apply rt1n_refl.
-  - apply rt1n_trans with (mApp t1 t2 (l ++ u :: l0)) ; try apply rt1n_refl.
-    + constructor. right. now constructor. 
-Qed.
-
-Local Hint Resolve up_subst_is_closed : core.
-
-Lemma two_subst_multistep :
-  forall t, is_canonical t -> forall σ, is_canonical_subst σ -> LambdaM.multistep t.[σ] t.{σ}.
-Proof.
-  pose LambdaM.multistep_is_compatible as H. destruct H.
-
-  intros t it.  
-  induction it using sim_is_canonical_ind
-    with (P0 := fun l (_: is_canonical_list l) => forall σ, is_canonical_subst σ -> LambdaM.multistep' l..[σ] l..{σ}) ; intros ; asimpl ;
-    try constructor ; auto.
-
-  - eapply multistep_trans ; fold LambdaM.multistep ; eauto.
-    eapply multistep_trans ; fold LambdaM.multistep ; eauto.
-    apply mApp_multistep_to_app.
-
-  - eapply multistep_trans ; fold LambdaM.multistep ; eauto.
-    eapply multistep_trans ; fold LambdaM.multistep ; eauto.
-    
-  - eapply multistep_trans ; fold LambdaM.multistep' ; eauto.
-Qed.
-
 Lemma conservativeness1 :
-  (forall (t t': Canonical.term), Canonical.step t t' -> LambdaM.multistep (i t) (i t'))
+  (forall (t t': Canonical.term), Canonical.step t t' -> LambdaM.multistep (ι t) (ι t'))
   /\
-  (forall l l', Canonical.step' l l' -> LambdaM.multistep' (map i l) (map i l')).
+  (forall l l', Canonical.step' l l' -> LambdaM.multistep' (map ι l) (map ι l')).
 Proof.
   pose LambdaM.multistep_is_compatible as H. destruct H.
 
@@ -60,53 +22,31 @@ Proof.
 
     (* reproduzir Beta1 em λm *)
     + inversion Beta1 ; subst. asimpl.
-      apply rt1n_trans with ((i t0).[(i u)/]).
+      apply rt1n_trans with (ι t0).[(ι u)/].
       * unfold LambdaM.step. constructor. left. left.
         now constructor. 
-      * rewrite (proj1 i_subst_pres). rewrite<- i_simple_subst.
-        apply two_subst_multistep.
-        ** apply i_image_is_canonical.
-        ** autounfold.
-           destruct x ; asimpl ; try easy.
-           *** apply i_image_is_canonical.
+      * apply multistep_H_inclusion.
+        rewrite ι_subst_rw. apply ι_subst_pres.
 
     (* reproduzir Beta2 em λm *)
     + inversion Beta2 ; subst. asimpl.
-      apply rt1n_trans with (mApp ((i t0).[(i u)/]) (i v) (map i l)).
-      * unfold LambdaM.step. constructor. left. right.
-        now constructor. 
-      * apply multistep_trans with (mApp (i t0.[u/]) (i v) (map i l)).
-        ** apply comp_mApp1.
-           rewrite (proj1 i_subst_pres).
-           rewrite<- i_simple_subst.
-           apply two_subst_multistep.
-           *** apply i_image_is_canonical.
-           *** autounfold.
-               destruct x ; asimpl ; try easy.
-               **** apply i_image_is_canonical.
-        ** destruct (t0.[u/]) ; asimpl in * ; subst ; try apply rt1n_refl.
-           *** apply rt1n_trans with (mApp (Var x) (i t) (map i (l0 ++ v :: l))) ; try easy.
-               **** constructor. right. constructor. now apply map_app.
-               **** constructor.
-           *** apply rt1n_trans with (mApp (Lam (i t)) (i t1) (map i (l0 ++ v :: l))).
-               **** constructor. right. constructor. apply map_app.
-               **** constructor.
-Qed.
+      apply rt1n_trans with (mApp ((ι t0).[(ι u)/]) (ι v) (map ι l)).
+      * constructor. left. right. now constructor. 
 
-Lemma h_subst_eq :
-  (forall (t: LambdaM.term) σ, h t.[σ] = (h t).[σ >>> h])
-  /\
-  (forall (l: list LambdaM.term) σ, map h l..[σ] = (map h l)..[σ >>> h]).
-Proof.
-  apply LambdaM.mut_term_ind ; intros ; asimpl ; f_equal ; try easy.
-  - now rewrite<- h_up_subst.
-  - rewrite H, H0, H1. now rewrite app_subst_pres.
+      * apply multistep_trans with (mApp (ι t0.[u/]) (ι v) (map ι l)).
+        ** apply comp_mApp1.
+           apply multistep_H_inclusion.
+           rewrite ι_subst_rw. apply ι_subst_pres.
+
+        ** rewrite ι_app_pres. 
+           apply multistep_H_inclusion.
+           apply app_is_multistep_H.
 Qed.
 
 Lemma conservativeness2 :
-  (forall (t t': LambdaM.term), LambdaM.step t t' -> Canonical.multistep (h t) (h t'))
+  (forall (t t': LambdaM.term), LambdaM.step t t' -> Canonical.multistep (π t) (π t'))
   /\
-  (forall (l l': list LambdaM.term), LambdaM.step' l l' -> Canonical.multistep' (map h l) (map h l')).
+  (forall (l l': list LambdaM.term), LambdaM.step' l l' -> Canonical.multistep' (map π l) (map π l')).
 Proof.
   pose Canonical.multistep_is_compatible as H. destruct H.
 
@@ -120,21 +60,22 @@ Proof.
     (* h preserva passos Beta *)
     + inversion Beta as [Beta1 | Beta2].
       * inversion Beta1 ; subst ; asimpl.
-        apply rt1n_trans with ((h t0).[h u/]).
+        apply rt1n_trans with ((π t0).[π u/]).
         ** constructor. left. now constructor. 
-        ** rewrite (proj1 h_subst_eq).
-           rewrite h_simple_subst. constructor.
+        ** rewrite (proj1 π_subst_pres).
+           rewrite π_subst_rw. constructor.
       * inversion Beta2 ; subst ; asimpl.
-        apply rt1n_trans with ((h t0).[h u/]@(h v, map h l)).
+        apply rt1n_trans with ((π t0).[π u/]@(π v, map π l)).
         ** constructor. right. now constructor. 
         ** apply multistep_comp_app1.
-           rewrite (proj1 h_subst_eq).
-           rewrite h_simple_subst. constructor.
+           rewrite (proj1 π_subst_pres).
+           rewrite π_subst_rw. constructor.
 
     (* h colapsa passos H *)
     + inversion H ; subst ; asimpl.
       (* aqui talvez fosse importante um lema! *)
-      destruct (h t0) ; asimpl ; rewrite map_app ; try constructor.
+      destruct (π t0) ; asimpl ;
+        rewrite map_app ; try constructor.
       * rewrite<- app_assoc. asimpl. constructor.
       * rewrite<- app_assoc. asimpl. constructor.
 Qed.
@@ -143,19 +84,19 @@ Qed.
 (* --------------------------- *)
 
 Theorem conservativeness :
-  forall t t', Canonical.multistep t t' <-> LambdaM.multistep (i t) (i t').
+  forall t t', Canonical.multistep t t' <-> LambdaM.multistep (ι t) (ι t').
 Proof.
   split.
   - intro H.
     induction H as [| t1 t2 t3].
     + constructor.
-    + apply multistep_trans with (i t2) ; try easy.
+    + apply multistep_trans with (ι t2) ; try easy.
       * now apply conservativeness1. 
   - intro H.
     rewrite<- (proj1 inversion2) with t.
     rewrite<- (proj1 inversion2) with t'.
     induction H as [| t1 t2 t3].
     + constructor.
-    + apply multistep_trans with (h t2) ; try easy.
+    + apply multistep_trans with (π t2) ; try easy.
       * now apply conservativeness2. 
 Qed.
