theories/MyRelations.v
@@ -1,0 +1,12 @@
+From Coq Require Import Relations.Relation_Definitions.
+From Coq Require Import Relations.Relation_Operators.
+
+Proposition multistep_trans (A: Type) (R: relation A):
+  forall x y z, clos_refl_trans_1n _ R x y -> clos_refl_trans_1n _ R y z ->
+            clos_refl_trans_1n _ R x z.
+Proof.                                                  
+  intros.
+  induction H.
+  - easy.
+  - eapply rt1n_trans ; eauto.
+Qed.
